better specs for complete and partial cursors. changing btnode_rep. adapting some proofs

verif/relation_mem.c
@@ -217,10 +217,7 @@ Cursor_T RL_NewCursor(Relation_T relation) {
     cursor->relation = relation;
     cursor->level = -1;
     moveToFirst(relation->root, cursor, 0);
-    for (i = cursor->level+1; i < MAX_TREE_DEPTH; i++) {
-        cursor->ancestorsIdx[i] = 0;
-        cursor->ancestors[i] = NULL;
-    }
+    
     return cursor;
 }
 
