verif/verif_currnode.v
@@ -21,31 +21,38 @@ Proof.
   start_function.
   destruct r as [[[root numRec] depth] prel].
   pose (r:=(root,numRec,depth,prel)).
+  destruct c as [|[n i] c'].
+  { destruct H; inv H; inv H1. inv H. } (* cursor can't be empty *)
+
   unfold cursor_rep. Intros anc_end. Intros idx_end.
+  assert_PROP( is_pointer_or_null (getval n)).
+  { assert(subnode (currNode ((n,i)::c') r) (get_root r)).
+    - destruct H.
+      + apply partial_cursor_subnode. inv H. auto.
+      + apply complete_cursor_subnode. inv H. auto.
+    - unfold get_root in H0. simpl in H0.
+      unfold relation_rep. rewrite subnode_rep with (n:=n) by auto. entailer!. }
   forward.                      (* t'1=cursor->level *)
   forward.                      (* t'2=cursor->ancestors[t'1] *)
-  entailer!. inv H. split. omega. rewrite MTD_eq in H9. assert (Z.of_nat 20 = 20). simpl. auto. omega.
-  (* TODO: rep_omega? *)
-  destruct c as [|[n i] c']. { inv H. inv H0. } assert_PROP( is_pointer_or_null (getval n)).
-  { apply cursor_rel_subnode in H0. unfold get_root in H0. simpl in H0.
-    unfold relation_rep. rewrite subnode_rep with (n:=n) by auto. entailer!. }
-  - entailer!. 
-    rewrite app_Znth1.
-    assert((Zlength ((n, i) :: c') - 1) = Zlength c').
-    rewrite Zlength_cons. rep_omega. rewrite H9.
-    rewrite app_Znth2. rewrite Zlength_rev. rewrite Zlength_map. rewrite Zlength_map.
-    assert (Zlength c' - Zlength c' = 0) by omega. rewrite H10. rewrite Znth_0_cons. auto.
+  { entailer!. apply partial_complete_length with (r:=r). auto. }
+  { entailer!. 
+    rewrite app_Znth1. rewrite app_Znth2.
+    rewrite Zlength_cons. rewrite Zsuccminusone. rewrite Zlength_rev. rewrite Zlength_map.
+    rewrite Zlength_map. assert(Zlength c'-Zlength c' = 0) by omega. rewrite H8.
+    rewrite Znth_0_cons. auto.
+    rewrite Zlength_cons. rewrite Zsuccminusone. rewrite Zlength_rev. rewrite Zlength_map.
+    rewrite Zlength_map. omega.
+    rewrite Zlength_cons. rewrite Zsuccminusone. rewrite Zlength_app. rewrite Zlength_rev.
+    rewrite Zlength_map. rewrite Zlength_map. rewrite Zlength_cons. simpl. omega. }
+  forward. entailer!.
+  + rewrite app_Znth1.
+    rewrite Zlength_cons. rewrite app_Znth2.
+    rewrite Zlength_rev. rewrite Zlength_map. rewrite Zlength_map.
+    assert((Z.succ (Zlength c') - 1 - Zlength c') = 0) by omega. rewrite H9.
+    rewrite Znth_0_cons. auto.
     rewrite Zlength_rev. rewrite Zlength_map. rewrite Zlength_map. omega.
     rewrite Zlength_app. rewrite Zlength_rev. rewrite Zlength_map. rewrite Zlength_map.
-    rewrite Zlength_cons. rewrite Zlength_cons. simpl. omega.
-  - forward. entailer!.
-    + rewrite app_Znth1. destruct c. inv H. inv H9.
-      rewrite Zlength_cons. simpl. destruct p. rewrite app_Znth2. simpl.
-      rewrite Zlength_rev. rewrite Zlength_map. rewrite Zlength_map.
-      assert((Z.succ (Zlength c) - 1 - Zlength c) = 0) by omega. rewrite H9. rewrite Znth_0_cons. auto.
-      rewrite Zlength_rev. rewrite Zlength_map. rewrite Zlength_map. omega.
-      rewrite Zlength_rev. rewrite Zlength_map. rewrite Zlength_map. omega.
-    + unfold cursor_rep. Exists anc_end. Exists idx_end.
-      cancel.
+    rewrite Zlength_cons. rewrite Zsuccminusone. rewrite Zlength_cons. simpl. omega.
+  + unfold cursor_rep. Exists anc_end. Exists idx_end.
+    cancel.
 Qed.
-
