verif/verif_entryindex.v
@@ -15,11 +15,12 @@ Require Import btrees.
 Require Import btrees_sep.
 Require Import btrees_spec.
 
-Lemma Znth_rev_cons: forall p (c:list val),
-    Znth (Zlength c) (rev (p::c)) = p.
+Lemma Znth_rev_cons: forall p (c:list val) d,
+    d = Zlength c -> 
+    Znth d (rev (p::c)) = p.
 Proof.
   intros.
-  induction c.
+  induction c; subst.
   - simpl. auto.
   - simpl. assert (Zlength (a::c) = Zlength c +1) by apply Zlength_cons. rewrite H.
     rewrite <- app_assoc. rewrite app_Znth2.
@@ -40,29 +41,26 @@ Proof.
   pose (r:=(root,numRec,depth,prel)).
   unfold cursor_rep. Intros anc_end. Intros Idx_end.
   forward.                      (* t'1=cursor->level *)
-  destruct c.
-  - inversion H. inversion H0.
+  destruct c as [|[n i ]c'].
+  - inv H; inv H0; inv H1. inv H0. (* no empty cursor *)
   - forward.                      (* t'2=cursor->ancestorsIdx[t'1] *)
     + entailer!.
-      unfold cursor_wf in H. destruct H.
-      split. omega.
-      assert (20=Z.of_nat MaxTreeDepth). rewrite MTD_eq. simpl. auto.
-      rewrite H8. omega.
+      apply partial_complete_length in H. auto.
     + entailer!. autorewrite with sublist.
-      assert (Z.succ (Zlength c) -1 - Zlength c = 0) by omega.
+      assert (Z.succ (Zlength c') -1 - Zlength c' = 0) by omega.
       rewrite H7. unfold Znth. simpl.
-      unfold rep_index. destruct (snd p); auto.
+      unfold rep_index. destruct i; auto.
     + autorewrite with sublist. deadvars!.
-      destruct r. destruct p. destruct p0. autorewrite with norm.
-      assert(Z.succ (Zlength c) -1 = Zlength c) by omega. rewrite H0.
-      pose (c':=map (fun x : node val * index.index => rep_index (snd x)) c). fold c'.
-      assert (Zlength c = Zlength c') by (unfold c'; rewrite Zlength_map; auto).
-      rewrite H1.
-      rewrite Znth_rev_cons.
+      destruct r. autorewrite with norm.
+      assert(Z.succ (Zlength c') -1 = Zlength c') by omega. rewrite H0.
+      pose (c'':=map (fun x : node val * index.index => rep_index (snd x)) c'). fold c''.
+      assert (Zlength c'' = Zlength c') by (unfold c''; rewrite Zlength_map; auto).
+      rewrite <- H1.
+      rewrite Znth_rev_cons by auto.
       forward. cancel.
       unfold cursor_rep.
       Exists (anc_end). Exists (Idx_end). cancel.
-      rewrite <- H1. assert (Zlength ((n, i) :: c) - 1 = Zlength c).
+      rewrite H1. assert (Zlength ((n, i) :: c') - 1 = Zlength c').
       rewrite Zlength_cons. omega. rewrite H10.
       cancel.
 Qed.
